\documentclass[a4paper, 12pt, titlepage]{article}

\input{include/base}
\input{include/font}
\input{include/commands}
\input{include/en}

\begin{document}
%% 中文习惯是设定首行缩进为2em. 注意此设置一定要在document环境之中, 这可能与\setlength作用范围相关
\setlength{\parindent}{2em}

% \title{A Test XeLaTex Document}
% \author{Jiayuan MAO}
% \maketitle

% \tableofcontents
% \listoffigures
% \listoftables

\paragraph{Subproblem 1.} \quad\par
\[ \Pr[X=k] = \binom{n}{k}~p^k (1-p)^{n-k} \]

\paragraph{Subproblem 2.} \quad\par
\[ \Pr[X=k \wedge N=n] = \frac{e^{-\lambda}\lambda^n}{n!}~\binom{n}{k} ~p^k (1-p)^{n-k} \]

\paragraph{Subproblem 4.} \quad\par
Here's a brief proof of the conclusion you used in your solution.

\begin{proof}
Prove by calculation.

\begin{eqnarray*}
	\E[X] & = & \sum_{n=1}^{\infty} \Pr[N=n] \sum_{k=1}^{\infty} \Pr[X=k\big|N=n]\\
	& = & \sum_{n=1}^{\infty} \Pr[N=n] \sum_{k=1}^{\infty} N p\\
	& = & \lambda \cdot p
\end{eqnarray*}

\end{proof}

\paragraph{Bonus} \quad\par
\begin{eqnarray*}
	\Pr[X=k] & = & \sum_{n=k}^{\infty} \frac{e^{-\lambda}\lambda^n}{n!}~\binom{n}{k} ~p^k (1-p)^{n-k}\\
	& = & e^{-\lambda} \sum_{n=k}^{\infty} \frac{\lambda^n}{n!} \cdot \frac{n!}{k!(n-k)!} \cdot p^k (1-p)^{n-k}\\
	& = & \frac{e^{-\lambda}}{k!} p^k (1-p)^{-k} \sum_{n=k}^{\infty} \frac{[\lambda(1-p) ]^n}{(n-k)!}\\
	& = & \frac{e^{-\lambda}}{k!} p^k (1-p)^{-k} \cdot [\lambda(1-p) ]^k \sum_{n=0}^{\infty} \frac{[\lambda(1-p) ]^n}{n!}\\
	& = & \frac{e^{-\lambda}}{k!} p^k (1-p)^{-k} \cdot [\lambda(1-p) ]^k \cdot e^{\lambda (-(p-1))}\\
	& = & \frac{\lambda ^k~p^k~e^{-p\lambda}}{k!}
\end{eqnarray*}

\[ \sum_{n=0}^\infty \frac{x^n}{n!} = e^x\]

\end{document}